## Rechengesetze (Kapitel 1)

| Gesetz | **Omega** = {1, 2, 3, 4, 5, 6}, **X** = {1, 3, 5, 6}, **Y** = {2, 3, 4, 5}, Z = {1} | Name |
| :-- | :-- | :-- |
| **X ∪ Y = Y ∪ X** | **\{1, 3, 5, 6\} ∪ \{2, 3, 4, 5\} = \{1, 2, 3, 4, 5, 6\} = \{2, 3, 4, 5\} ∪ \{1, 3, 5, 6\}** | Kommutativgesetze |
| **X ∩ Y = Y ∩ X** | **\{1, 3, 5, 6\} ∩ \{2, 3, 4, 5\} = \{3, 5\} = \{2, 3, 4, 5\} ∩ \{1, 3, 5, 6\}** | Kommutativgesetze |
| **(X ∪ Y) ∪ Z = X ∪ (Y ∪ Z)** | **(\{1, 3, 5, 6\} ∪ \{2, 3, 4, 5\}) ∪ \{1\} = \{1, 2, 3, 4, 5, 6\} = \{1, 3, 5, 6\} ∪ (\{2, 3, 4, 5\} ∪ \{1\})** | Assoziativgesetze |
| **(X ∩ Y) ∩ Z = X ∩ (Y ∩ Z)** | **(\{1, 3, 5, 6\} ∩ \{2, 3, 4, 5\}) ∩ \{1\} = ∅ = \{1, 3, 5, 6\} ∩ (\{2, 3, 4, 5\} ∩ \{1\})** | Assoziativgesetze |
| **(X ∪ Y) ∩ Z = (X ∩ Z) ∪ (Y ∩ Z)** | **(\{1, 3, 5, 6\} ∪ \{2, 3, 4, 5\}) ∩ \{1\} = \{1\} = (\{1, 3, 5, 6\} ∩ \{1\}) ∪ (\{2, 3, 4, 5\} ∩ \{1\})** | Distributivgesetze |
| **(X ∩ Y) ∪ Z = (X ∪ Z) ∩ (Y ∪ Z)** | **(\{1, 3, 5, 6\} ∩ \{2, 3, 4, 5\}) ∪ \{1\} = \{1, 3, 5\} = (\{1, 3, 5, 6\} ∪ \{1\}) ∩ (\{2, 3, 4, 5\} ∪ \{1\})** | Distributivgesetze |
| **X ∪ (X ∩ Y) = X** | **\{1, 3, 5, 6\} ∪ (\{1, 3, 5, 6\} ∩ \{2, 3, 4, 5\}) = \{1, 3, 5, 6\} ∪ \{3, 5\} = \{1, 3, 5, 6\}** | Absorptionsgesetze |
| **X ∩ (X ∪ Y) = X** | **\{1, 3, 5, 6\} ∩ (\{1, 3, 5, 6\} ∪ \{2, 3, 4, 5\}) = \{1, 3, 5, 6\} ∩ \{1, 2, 3, 4, 5, 6\} = \{1, 3, 5, 6\}** | Absorptionsgesetze |
| **¬{X ∪ Y} = ¬{X} ∩ ¬{Y}** | **Ω = (\{1, 3, 5, 6\} ∪ \{2, 3, 4, 5\}) = ∅ = (Ω = \{1, 3, 5, 6\}) ∩ (Ω = \{2, 3, 4, 5\}) = \{2, 4\} ∩ \{1, 6\} = ∅** | Gesetze von de Morgan |
| **¬{X ∩ Y} = ¬{X} ∪ ¬{Y}** | **Ω = (\{1, 3, 5, 6\} ∩ \{2, 3, 4, 5\}) = \{1, 2, 4, 6\} = (Ω = \{1, 3, 5, 6\}) ∪ (Ω = \{2, 3, 4, 5\}) = \{2, 4\} ∪ \{1, 6\}** | Gesetze von de Morgan |
